Now we obtain the Fermat principle because $k^i = \text{grad} \psi$:
\begin{equation*}
	 \oint \text{grad} \psi \d \vc{l} = \oint n \vc{s} \d \vc{l} = 0 
	 \hspace{1 cm}
	\Leftrightarrow
	\hspace{1 cm}
	\delta \int n \d l = 0.
\end{equation*}
We will consider that 
\begin{equation*}
	d l = \sqrt{ d x^2 + d y^2} = \sqrt{1 + (y_x')^2} \d x
	\hspace{0.5 cm}
	\Rightarrow
	\hspace{0.5 cm}
	\delta \int n \sqrt{1 + (y_x')^2} \d x = 0.
\end{equation*}
So it is Euler-Lagrange equation and the path of light is well known
\begin{equation*}
	\frac{d}{d x} \frac{\partial L}{\partial y_x'} - \frac{\partial L}{\partial y} = 0,
	\hspace{0.5 cm}
	\text{for } L = n \sqrt{1 + (y_x')^2}.
\end{equation*}