\subsubsection*{Т25}

Теперь найдём предел вида
\begin{equation*}
    * w. \lim_{n\to \infty} \frac{n^3 x}{(1+n^2 x^2)^2} = 
    * w. \lim_{a \to +0} \frac{x a}{(x^2+a^2)^2} = F,
\end{equation*}
для этого 
\begin{equation*}
    \bigg\langle \frac{xa}{(x^2+a^2)^2} \,\bigg|\, \varphi \bigg\rangle  = 
    \int_{-\infty}^{+\infty} \frac{xa}{(x^2+a^2)^2} \varphi(x) \d x = \int_{-\infty}^{+\infty} 
    \left(-\frac{1}{2}\right)\left(
        \frac{\partial }{\partial x} \frac{a}{x^2 + a^2}
    \right) \varphi(x) \d x = 
    \frac{1}{2} \int_{-\infty}^{+\infty}  \frac{a \varphi'(x)}{x^2 + a^2} \d x \underset{a\to+0}{\to} \frac{\pi}{2} \varphi'(0),
\end{equation*}
что, учитывая предыдущую задачу, позволяет записать
\begin{equation*}
     \frac{\pi}{2} \langle \delta(x) \,|\, \varphi' \rangle = \bigg\langle \left(-\frac{\pi}{2}\right)\delta'(x)   \,\bigg|\, \varphi \bigg\rangle,
     \hspace{0.5cm} \Rightarrow \hspace{0.5cm}
     w. \lim_{a \to +0} \frac{x a}{(x^2+a^2)^2}  = -\frac{\pi}{2}\delta'(x), 
\end{equation*}