\subsubsection*{Дополнительная задача о \texorpdfstring{$\cos e^{ix}$}{2}}

Найдём суммы вида
\begin{equation*}
    \sum_{n=0}^{\infty} \left(
        (-1)^n \frac{\cos (2nx)}{(2n)!} + i (-1)^n \frac{\sin(2nx)}{(2n)!}
    \right) = \sum_{n=0}^{\infty} \frac{(-1)^n e^{2inx}}{(2n)!},
\end{equation*}
далее, принимая $z = e^{ix}$, найдём по определению
\begin{equation*}
    \sum_{n=0}^{\infty} \frac{(-1)^n e^{2inx}}{(2n)!} = 
    \frac{(-1)^n z^{2n}}{(2n)!} = \cos \left(
        z
    \right) = \cos \left(e^{ix}\right).
\end{equation*}