\subsection*{У2}
\begin{itemize}
	\item $[\vc{a} \times [\vc{b} \times \vc{c}]]^i = \varepsilon_{\phantom{0} j k}^{i} a^j [\vc{b} \times \vc{c}]^k
	=
	\varepsilon_{\phantom{0} j k}^i a^j \varepsilon_{\phantom{0} m n}^k b^m c^n = \left(\delta_{m}^{i} \delta_{j n} - \delta_{n}^{i} \delta_{j m} \right) a^j b^m c^n
	=
	a^j b^i c_j - c^i a^j b_j
	=
	b^i (\vc{a} \cdot \vc{c}) - c^i (\vc{a} \cdot \vc{b}).$

	\item $\left([\vc{a} \times \vc{b}] \cdot [\vc{c} \times \vc{d}]\right)
	=
	\varepsilon_{i j k} a^j b^k \varepsilon_{\phantom{0} m n}^{i} c^m d^n
	= \left(\delta_{j m} \delta_{k n} - \delta_{j n} \delta_{k m} \right) a^j b^k c^m d^n
	= a^j b^k c_j d_k - a^j b^k c_k d_j
	=$

	$=(\vc{a} \cdot \vc{c})(\vc{b} \cdot \vc{d}) - (\vc{a} \cdot \vc{d})(\vc{b} \cdot \vc{c}).$

	\item Тут придется применить результаты первого примера этого урпажения:
	\begin{equation*}
	\left([\vc{a} \times \vc{b}] \cdot [ [\vc{b} \times \vc{c}] \times [\vc{c} \times \vc{a}] ]\right)
	=
	\left(\vc{a} \cdot [\vc{b} \times \vc{c}]\right) \left(\vc{b} \cdot [\vc{c} \times \vc{a}]\right)
	-
	\left(\vc{a} \cdot [\vc{c} \times \vc{a}]\right) \left(\vc{b} \cdot [\vc{b} \times \vc{c}]\right)
	=
\end{equation*}	
\begin{equation*}
	=
	a^i \varepsilon_{i j k} b^j c^k \cdot b^{\alpha} \varepsilon_{\alpha \beta \gamma} c^\beta a^\gamma 
	-
	a^i \varepsilon_{i j k} c^j a^k \cdot b^{\alpha} \varepsilon_{\alpha \beta \gamma} b^\beta c^\gamma
	= (a^i \varepsilon_{i j k} b^j c^k)^2 = \left(\vc{a} \cdot [\vc{b} \times \vc{c}]\right)^2	
\end{equation*}
\end{itemize}

% \begin{equation*}
% 	[\vc{a} \times [\vc{b} \times \vc{c}]]^i = \varepsilon_{\phantom{0} j k}^{i} a^j [\vc{b} \times \vc{c}]^k
% 	=
% 	\varepsilon_{\phantom{0} j k}^i a^j \varepsilon_{\phantom{0} m n}^k b^m c^n = \left(\delta_{m}^{i} \delta_{j n} - \delta_{n}^{i} \delta_{j m} \right) a^j b^m c^n
% 	=
% 	a^j b^i c_j - c^i a^j b_j
% 	=
% 	b^i (\vc{a} \cdot \vc{c}) - c^i (\vc{a} \cdot \vc{b}).
% \end{equation*}

% \begin{equation*}
% 	\left([\vc{a} \times \vc{b}] \cdot [\vc{c} \times \vc{d}]\right)
% 	=
% 	\varepsilon_{i j k} a^j b^k \varepsilon_{\phantom{0} m n}^{i} c^m d^n
% 	= \left(\delta_{j m} \delta_{k n} - \delta_{j n} \delta_{k m} \right) a^j b^k c^m d^n
% 	= a^j b^k c_j d_k - a^j b^k c_k d_j
% 	=
% 	(\vc{a} \cdot \vc{c})(\vc{b} \cdot \vc{d}) - (\vc{a} \cdot \vc{d})(\vc{b} \cdot \vc{c}).
% \end{equation*}

% Тут придется применить результаты первого примера этого урпажения:
% \begin{equation*}
% 	\left([\vc{a} \times \vc{b}] \cdot [ [\vc{b} \times \vc{c}] \times [\vc{c} \times \vc{a}] ]\right)
% 	=
% 	\left(\vc{a} \cdot [\vc{b} \times \vc{c}]\right) \left(\vc{b} \cdot [\vc{c} \times \vc{a}]\right)
% 	-
% 	\left(\vc{a} \cdot [\vc{c} \times \vc{a}]\right) \left(\vc{b} \cdot [\vc{b} \times \vc{c}]\right)
% 	=
% \end{equation*}	
% \begin{equation*}
% 	=
% 	a^i \varepsilon_{i j k} b^j c^k \cdot b^{\alpha} \varepsilon_{\alpha \beta \gamma} c^\beta a^\gamma 
% 	-
% 	a^i \varepsilon_{i j k} c^j a^k \cdot b^{\alpha} \varepsilon_{\alpha \beta \gamma} b^\beta c^\gamma
% 	= (a^i \varepsilon_{i j k} b^j c^k)^2 = \left(\vc{a} \cdot [\vc{b} \times \vc{c}]\right)^2	
% \end{equation*}